Haskell version of probability theory

opentheory/theories/probability/probability.ml
@@ -23,53 +23,52 @@ export_thm dest_mk_random;;
 
 let random_tybij = CONJ mk_dest_random dest_mk_random;;
 
-let rbit_def = new_definition
-  `!r. rbit r = (shd (dest_random r), mk_random (stl (dest_random r)))`;;
+let random_bit_def = new_definition
+  `!r. random_bit r = shd (dest_random r)`;;
 
-export_thm rbit_def;;
+export_thm random_bit_def;;
 
-let rsplit_def = new_definition
+let split_random_def = new_definition
   `!r.
-     rsplit r =
+     split_random r =
      let (s1,s2) = ssplit (dest_random r) in
      (mk_random s1, mk_random s2)`;;
 
-export_thm rsplit_def;;
+export_thm split_random_def;;
 
-let (rdecode_vector_zero,rdecode_vector_suc) =
+let (random_vector_zero,random_vector_suc) =
   let def = new_recursive_definition num_RECURSION
-    `(!(d : random -> A # random) r. rdecode_vector d 0 r = ([],r)) /\
-     (!d r n.
-        rdecode_vector d (SUC n) r =
-        let (h,r') = d r in
-        let (t,r'') = rdecode_vector d n r' in
-        (CONS h t, r''))` in
+    `(!(f : random -> A) r. random_vector f 0 r = []) /\
+     (!f r n.
+        random_vector f (SUC n) r =
+        let (r1,r2) = split_random r in
+        CONS (f r1) (random_vector f n r2))` in
   CONJ_PAIR def;;
 
-export_thm rdecode_vector_zero;;
-export_thm rdecode_vector_suc;;
+export_thm random_vector_zero;;
+export_thm random_vector_suc;;
 
-let rdecode_vector_def = CONJ rdecode_vector_zero rdecode_vector_suc;;
+let random_vector_def = CONJ random_vector_zero random_vector_suc;;
 
-let rbits_def = new_definition
-  `rbits = rdecode_vector rbit`;;
+let random_bits_def = new_definition
+  `random_bits = random_vector random_bit`;;
 
-export_thm rbits_def;;
+export_thm random_bits_def;;
 
-let rdecode_geometric_loop_exists = prove
+let random_geometric_loop_exists = prove
  (`?loop. !n r.
      loop n r =
-       let (b,r') = rbit r in
-       if b then n else
-       loop (SUC n) r'`,
+       let (r1,r2) = split_random r in
+       if random_bit r1 then n else
+       loop (SUC n) r2`,
   MP_TAC
    (ISPECL
       [`\ ((n : num), (r : random)).
-          let (b,r') = rbit r in
-          ~b`;
+          let (r1,r2) = split_random r in
+          ~random_bit r1`;
        `\ ((n : num), (r : random)).
-          let (b,r') = rbit r in
-          (SUC n, r')`;
+          let (r1,r2) = split_random r in
+          (SUC n, r2)`;
        `\ ((n : num), (r : random)).
           n`] WF_REC_TAIL) THEN
   DISCH_THEN
@@ -82,34 +81,31 @@ let rdecode_geometric_loop_exists = prove
   REWRITE_TAC [] THEN
   FIRST_X_ASSUM (fun th -> CONV_TAC (LAND_CONV (ONCE_REWRITE_CONV [th]))) THEN
   REWRITE_TAC [LET_DEF; LET_END_DEF] THEN
-  PAIR_CASES_TAC `rbit r` THEN
+  PAIR_CASES_TAC `split_random r` THEN
   DISCH_THEN
-    (X_CHOOSE_THEN `b : bool` (X_CHOOSE_THEN `r' : random` SUBST1_TAC)) THEN
+    (X_CHOOSE_THEN `r1 : random` (X_CHOOSE_THEN `r2 : random` SUBST1_TAC)) THEN
   REWRITE_TAC [] THEN
-  BOOL_CASES_TAC `b : bool` THEN
+  BOOL_CASES_TAC `random_bit r1` THEN
   REWRITE_TAC []);;
 
-let rdecode_geometric_loop_def =
-  new_specification ["rdecode_geometric_loop"]
-    rdecode_geometric_loop_exists;;
+let random_geometric_loop_def =
+  new_specification ["random_geometric_loop"]
+    random_geometric_loop_exists;;
 
-export_thm rdecode_geometric_loop_def;;
+export_thm random_geometric_loop_def;;
 
-let rdecode_geometric_def = new_definition
-  `!r.
-     rdecode_geometric r =
-     let (r1,r2) = rsplit r in
-     (rdecode_geometric_loop 0 r1, r2)`;;
+let random_geometric_def = new_definition
+  `random_geometric = random_geometric_loop 0`;;
 
-export_thm rdecode_geometric_def;;
+export_thm random_geometric_def;;
 
-let rdecode_list_def = new_definition
-  `!d r.
-     rdecode_list (d : random -> A # random) r =
-     let (n,r') = rdecode_geometric r in
-     rdecode_vector d n r'`;;
+let random_geometric_list_def = new_definition
+  `!f r.
+     random_geometric_list (f : random -> A) r =
+     let (r1,r2) = split_random r in
+     random_vector f (random_geometric r1) r2`;;
 
-export_thm rdecode_list_def;;
+export_thm random_geometric_list_def;;
 
 (* ------------------------------------------------------------------------- *)
 (* Properties of probability.                                                *)
@@ -117,30 +113,58 @@ export_thm rdecode_list_def;;
 
 logfile "probability-thm";;
 
-let length_rdecode_vector = prove
- (`!(d : random -> A # random) n r. LENGTH (FST (rdecode_vector d n r)) = n`,
+let length_random_vector = prove
+ (`!(f : random -> A) n r. LENGTH (random_vector f n r) = n`,
   GEN_TAC THEN
   INDUCT_TAC THENL
-  [REWRITE_TAC [rdecode_vector_def; LENGTH];
+  [REWRITE_TAC [random_vector_def; LENGTH];
    GEN_TAC THEN
-   PAIR_CASES_TAC `(d : random -> A # random) r` THEN
+   REWRITE_TAC [random_vector_def] THEN
+   PAIR_CASES_TAC `split_random r` THEN
    DISCH_THEN
-     (X_CHOOSE_THEN `h : A`
-       (X_CHOOSE_THEN `r' : random` STRIP_ASSUME_TAC)) THEN
-   PAIR_CASES_TAC `rdecode_vector (d : random -> A # random) n r'` THEN
-   DISCH_THEN
-     (X_CHOOSE_THEN `t : A list`
-       (X_CHOOSE_THEN `r'' : random` STRIP_ASSUME_TAC)) THEN
-   FIRST_X_ASSUM (MP_TAC o SPEC `r' : random`) THEN
-   ASM_REWRITE_TAC
-     [rdecode_vector_def; LENGTH; LET_DEF; LET_END_DEF; SUC_INJ]]);;
+     (X_CHOOSE_THEN `r1 : random`
+       (X_CHOOSE_THEN `r2 : random` STRIP_ASSUME_TAC)) THEN
+   ASM_REWRITE_TAC [LENGTH; LET_DEF; LET_END_DEF]]);;
 
-export_thm length_rdecode_vector;;
+export_thm length_random_vector;;
 
-let length_rbits = prove
- (`!n r. LENGTH (FST (rbits n r)) = n`,
-  REWRITE_TAC [rbits_def; length_rdecode_vector]);;
+let random_vector_src = prove
+ (`!(f : random -> A) n r.
+     random_vector f n r =
+     if n = 0 then [] else
+     let (r1,r2) = split_random r in
+     CONS (f r1) (random_vector f (n - 1) r2)`,
+  REPEAT GEN_TAC THEN
+  MP_TAC (SPEC `n : num` num_CASES) THEN
+  DISCH_THEN
+    (DISJ_CASES_THEN2
+       SUBST_VAR_TAC
+       (X_CHOOSE_THEN `m : num` SUBST_VAR_TAC)) THEN
+  REWRITE_TAC [random_vector_def; SUC_SUB1; NOT_SUC]);;
 
-export_thm length_rbits;;
+export_thm random_vector_src;;
+
+let length_random_bits = prove
+ (`!n r. LENGTH (random_bits n r) = n`,
+  REWRITE_TAC [random_bits_def; length_random_vector]);;
+
+export_thm length_random_bits;;
+
+let random_geometric_loop_src =
+    REWRITE_RULE [ADD1] random_geometric_loop_def;;
+
+export_thm random_geometric_loop_src;;
+
+(* ------------------------------------------------------------------------- *)
+(* Haskell source for probability.                                           *)
+(* ------------------------------------------------------------------------- *)
+
+logfile "probability-haskell-src";;
+
+export_thm random_vector_src;;  (* Haskell *)
+export_thm random_bits_def;;  (* Haskell *)
+export_thm random_geometric_loop_src;;  (* Haskell *)
+export_thm random_geometric_def;;  (* Haskell *)
+export_thm random_geometric_list_def;;  (* Haskell *)
 
 logfile_end ();;
